src/Ex/MsiSvInv.v
@@ -1,0 +1,2232 @@
+Require Import Bool List String Peano_dec Lia.
+Require Import Common FMap HVector Syntax Topology Semantics SemFacts StepM.
+Require Import Invariant TrsInv Simulation Serial SerialFacts.
+Require Import RqRsLang RqRsCorrect.
+
+Require Import Msi MsiSv SpecSv MsiSvTopo.
+
+Set Implicit Arguments.
+
+Import MonadNotations.
+Import CaseNotations.
+
+Open Scope list.
+Open Scope hvec.
+Open Scope fmap.
+
+Definition Mii := (IdxT * IdxT)%type.
+
+Definition mii_dec: forall mii1 mii2: Mii, {mii1 = mii2} + {mii1 <> mii2}.
+Proof.
+  decide equality.
+  - apply eq_nat_dec.
+  - apply eq_nat_dec.
+Defined.
+
+Definition miis_dec := list_eq_dec mii_dec.
+
+Definition miiOf (idm: Id Msg): Mii := (idOf idm, msg_id (valOf idm)).
+Definition miisOf (msgs: list (Id Msg)): list Mii :=
+  map miiOf msgs.
+
+Definition AtomicMsgOutsInv {oifc} (mp: MsgOutPred oifc)
+           (eouts: list (Id Msg)) (nst: MState oifc): Prop :=
+  Forall (fun eout => mp eout nst.(bst_oss) nst.(bst_orqs)) eouts.
+
+Definition AtomicLocksInv {oifc}
+           (lp: IdxT -> ORq Msg -> Prop)
+           (hst: MHistory) (nst: MState oifc): Prop :=
+  forall oidx,
+    In oidx (oindsOf hst) ->
+    orq <-- (bst_orqs nst)@[oidx]; lp oidx orq.
+
+Definition AtomicInv {oifc}
+           (mp: MsgOutPred oifc)
+           (lp: IdxT -> ORq Msg -> Prop):
+  list (Id Msg) (* inits *) ->
+  MState oifc (* starting state *) ->
+  MHistory (* atomic history *) ->
+  list (Id Msg) (* eouts *) ->
+  MState oifc (* ending state *) -> Prop :=
+  fun inits st1 hst eouts st2 =>
+    AtomicMsgOutsInv mp eouts st2 /\
+    AtomicLocksInv lp hst st2.
+
+Section Inv.
+
+  (** Basic predicates per an object *)
+  
+  Definition ImplOStateM (cv: nat) (ost: OState ImplOStateIfc): Prop :=
+    ost#[implStatusIdx] = msiM /\ ost#[implValueIdx] = cv.
+
+  Definition ImplOStateS (cv: nat) (ost: OState ImplOStateIfc): Prop :=
+    ost#[implStatusIdx] = msiS /\ ost#[implValueIdx] = cv.
+
+  Definition ImplOStateI (ost: OState ImplOStateIfc): Prop :=
+    ost#[implStatusIdx] = msiI.
+
+  Definition ImplOStateSI (cv: nat) (ost: OState ImplOStateIfc): Prop :=
+    ImplOStateS cv ost \/ ImplOStateI ost.
+
+  Definition ImplOStateMSI (cv: nat) (ost: OState ImplOStateIfc): Prop :=
+    ost#[implStatusIdx] >= msiS -> ost#[implValueIdx] = cv.
+
+  Definition ImplDirM (ost: OState ImplOStateIfc): Prop :=
+    (ost#[implDirIdx].(fst) = msiM /\ ost#[implDirIdx].(snd) = msiI) \/
+    (ost#[implDirIdx].(fst) = msiI /\ ost#[implDirIdx].(snd) = msiM).
+
+  Definition ImplDirS (ost: OState ImplOStateIfc): Prop :=
+    ost#[implDirIdx].(fst) <= msiS /\
+    ost#[implDirIdx].(snd) <= msiS.
+
+  Definition ImplDirI (ost: OState ImplOStateIfc): Prop :=
+    ost#[implDirIdx].(fst) = msiI /\
+    ost#[implDirIdx].(snd) = msiI.
+
+  Section GInv.
+    Variables (post cost1 cost2: OState ImplOStateIfc)
+              (porq corq1 corq2: ORq Msg).
+
+    (** The first invariant: the directory status is coherent to statuses of
+     * children. Note that an object is *not* required to keep the coherency
+     * when it is (properly) locked (the meaning of "properly" depends on the
+     * protocol).
+     *)
+    Definition ImplDirCoh: Prop :=
+      !porq@[downRq];
+        (!corq1@[upRq]; cost1#[implStatusIdx] = post#[implDirIdx].(fst)) /\
+        (!corq2@[upRq]; cost2#[implStatusIdx] = post#[implDirIdx].(snd)).
+    
+    (** The second invariant is only for parent, saying that the parent status
+     * and its directory status are coherent.
+     *)
+    Definition ImplParentCoh (cv: nat): Prop :=
+      !porq@[downRq];
+      ((ImplOStateM cv post /\ ImplDirI post) \/
+       (ImplOStateS cv post /\ ImplDirS post) \/
+       (ImplOStateI post /\ ImplDirM post)).
+
+    (** The last invariant is for children, in order for ensuring
+     * the local coherency. 
+     *)
+    Definition ImplChildCoh1 (cv: nat): Prop :=
+      !corq1@[upRq]; ImplOStateMSI cv cost1.
+    Definition ImplChildCoh2 (cv: nat): Prop :=
+      !corq2@[upRq]; ImplOStateMSI cv cost2.
+
+    Definition ImplChildrenCoh: Prop :=
+      !corq1@[upRq]; !corq2@[upRq];
+        (cost1#[implStatusIdx] = msiM -> cost2#[implStatusIdx] = msiI) /\
+        (cost2#[implStatusIdx] = msiM -> cost1#[implStatusIdx] = msiI).
+  
+    Definition ImplStateCoh (cv: nat): Prop :=
+      ImplParentCoh cv /\ 
+      ImplChildCoh1 cv /\ ImplChildCoh2 cv /\
+      ImplChildrenCoh.
+
+  End GInv.
+
+  Definition ImplStateInv (st: MState ImplOStateIfc): Prop :=
+    post <-- (bst_oss st)@[parentIdx];
+      cost1 <-- (bst_oss st)@[child1Idx];
+      cost2 <-- (bst_oss st)@[child2Idx];
+      porq <-- (bst_orqs st)@[parentIdx];
+      corq1 <-- (bst_orqs st)@[child1Idx];
+      corq2 <-- (bst_orqs st)@[child2Idx];
+      (exists cv, ImplStateCoh post cost1 cost2 porq corq1 corq2 cv) /\
+      (ImplDirCoh post cost1 cost2 porq corq1 corq2).
+
+  Hint Unfold ImplOStateM ImplOStateS ImplOStateI ImplOStateSI ImplOStateMSI
+       ImplDirM ImplDirS ImplDirI
+       ImplDirCoh ImplParentCoh ImplChildCoh1 ImplChildCoh2 ImplChildrenCoh
+       ImplStateCoh: RuleConds.
+
+  Ltac disc_msi :=
+    try
+      match goal with
+      | [H: ?t = ?t -> _ |- _] => specialize (H eq_refl)
+      | [H: ?p -> _, Hp: ?p |- _] => specialize (H Hp)
+      | [H: VNat ?v = VNat _ |- _] => is_var v; inv H
+      | [H: VNat _ = VNat ?v |- _] => is_var v; inv H
+      | [H: ?oss@[parentIdx] = Some ?ost |- _] =>
+        match type of ost with
+        | OState _ =>
+          let val := fresh "val" in
+          let stt := fresh "stt" in
+          let dir := fresh "dir" in
+          destruct ost as [val [stt [dir ?]]]
+        end
+      | [H: ?oss@[child1Idx] = Some ?ost |- _] =>
+        match type of ost with
+        | OState _ =>
+          let val := fresh "val" in
+          let stt := fresh "stt" in
+          destruct ost as [val [stt ?]]
+        end
+      | [H: ?oss@[child2Idx] = Some ?ost |- _] =>
+        match type of ost with
+        | OState _ =>
+          let val := fresh "val" in
+          let stt := fresh "stt" in
+          destruct ost as [val [stt ?]]
+        end
+      | [H: msiM = _ |- _] => apply eq_sym in H
+      | [H: msiS = _ |- _] => apply eq_sym in H
+      | [H: msiI = _ |- _] => apply eq_sym in H
+      | [H1: ?t = msiM, H2: ?t = msiS |- _] => rewrite H1 in H2; discriminate
+      | [H1: ?t = msiM, H2: ?t = msiI |- _] => rewrite H1 in H2; discriminate
+      | [H1: ?t = msiS, H2: ?t = msiI |- _] => rewrite H1 in H2; discriminate
+      | [H1: ?t = msiM, H2: ?t <= msiS |- _] =>
+        rewrite H1 in H2; unfold msiM, msiS in H2; lia
+      | [H1: ?t = msiI, H2: ?t >= msiS |- _] =>
+        rewrite H1 in H2; unfold msiS, msiI in H2; lia
+      end.
+
+  Ltac disc_rule_custom ::=
+    try disc_msi.
+  
+  Section Facts.
+
+    Lemma msiSv_impl_ORqsInit: GoodORqsInit (initsOf impl).
+    Proof.
+      red; intros.
+      cbn; unfold implORqsInit.
+      mred.
+    Qed.
+
+    Lemma implStateInv_orqs_weakened:
+      forall st oidx orq norq rqt rqi nmsgs,
+        ImplStateInv st ->
+        (bst_orqs st)@[oidx] = Some orq ->
+        norq = orq +[rqt <- rqi] ->
+        ImplStateInv {| bst_oss := bst_oss st;
+                        bst_orqs := (bst_orqs st) +[oidx <- norq];
+                        bst_msgs := nmsgs |}.
+    Proof.
+      unfold ImplStateInv; simpl; intros.
+      disc_rule_conds_const.
+      destruct H as [[cv ?] ?].
+      solve_rule_conds_ex.
+    Qed.
+
+    Lemma implStateCoh_M_value_changed:
+      forall st,
+        ImplStateInv st ->
+        forall oidx ost orq,
+          (oidx = child1Idx \/ oidx = child2Idx) ->
+          (bst_oss st)@[oidx] = Some ost ->
+          ost#[implStatusIdx] = msiM ->
+          (bst_orqs st)@[oidx] = Some orq ->
+          orq@[upRq] = None ->
+          forall n (uv: DirT * unit) nmsgs,
+            ImplStateInv
+              (Build_MState
+                 (oifc:= ImplOStateIfc)
+                 ((bst_oss st) +[oidx <- (n, (msiM, uv))])
+                 (bst_orqs st) nmsgs).
+    Proof.
+      unfold ImplStateInv; simpl; intros.
+      disc_rule_conds_const.
+      destruct H as [[cv ?] ?].
+      disc_rule_conds_ex.
+      - destruct H0; discriminate.
+      - split.
+        + exists n; repeat split.
+          * disc_rule_conds_ex.
+            destruct H as [|[|]]; try (exfalso; solve_rule_conds_ex; fail).
+            right; right.
+            solve_rule_conds_ex.
+          * solve_rule_conds_ex.
+            unfold msiM, msiS, msiI in *; lia.
+          * solve_rule_conds_ex.
+          * solve_rule_conds_ex.
+        + solve_rule_conds_ex.
+      - split.
+        + exists n; repeat split.
+          * disc_rule_conds_ex.
+            destruct H as [|[|]]; try (exfalso; solve_rule_conds_ex; fail).
+            right; right.
+            solve_rule_conds_ex.
+          * solve_rule_conds_ex.
+            unfold msiM, msiS, msiI in *; lia.
+          * solve_rule_conds_ex.
+          * solve_rule_conds_ex.
+        + solve_rule_conds_ex.
+      - eauto 6.
+    Qed.
+
+    Lemma msiSv_impl_InvTrs_ext_in:
+      forall st1 eins st2,
+        ImplStateInv st1 ->
+        step_m impl st1 (RlblIns eins) st2 ->
+        ImplStateInv st2.
+    Proof.
+      intros; inv_step; assumption.
+    Qed.
+
+    Lemma msiSv_impl_InvTrs_ext_out:
+      forall st1 eouts st2,
+        ImplStateInv st1 ->
+        step_m impl st1 (RlblOuts eouts) st2 ->
+        ImplStateInv st2.
+    Proof.
+      intros; inv_step; assumption.
+    Qed.
+
+    Definition MsiSvMsgOutPred: MsgOutPred ImplOStateIfc :=
+      fun eout oss orqs =>
+        match case (miiOf eout) on mii_dec default True with
+        | (ec1, Spec.getRq): False
+        | (ec1, Spec.setRq): False
+        | (ec1, Spec.evictRq): False
+        | (ec2, Spec.getRq): False
+        | (ec2, Spec.setRq): False
+        | (ec2, Spec.evictRq): False
+
+        | (pc1, msiRsS): 
+            post <-- oss@[parentIdx];
+            porq <-- orqs@[parentIdx];
+            post#[implStatusIdx] = msiS /\
+            post#[implDirIdx].(fst) = msiS /\
+            porq@[downRq] = None /\
+            msg_value (valOf eout) = VNat post#[implValueIdx]
+        | (pc2, msiRsS):
+            post <-- oss@[parentIdx];
+            porq <-- orqs@[parentIdx];
+            post#[implStatusIdx] = msiS /\
+            post#[implDirIdx].(snd) = msiS /\
+            porq@[downRq] = None /\
+            msg_value (valOf eout) = VNat post#[implValueIdx]
+
+        | (pc1, msiRsM):
+            post <-- oss@[parentIdx];
+            porq <-- orqs@[parentIdx];
+            post#[implStatusIdx] = msiI /\
+            post#[implDirIdx].(fst) = msiM /\
+            porq@[downRq] = None
+        | (pc2, msiRsM):
+            post <-- oss@[parentIdx];
+            porq <-- orqs@[parentIdx];
+            post#[implStatusIdx] = msiI /\
+            post#[implDirIdx].(snd) = msiM /\
+            porq@[downRq] = None
+
+        | (pc1, msiRsI):
+            post <-- oss@[parentIdx];
+            ((post#[implStatusIdx] = msiM /\
+              post#[implDirIdx].(fst) = msiI) \/
+             (post#[implStatusIdx] = msiS /\
+              post#[implDirIdx].(fst) = msiI))
+        | (pc2, msiRsI):
+            post <-- oss@[parentIdx];
+            ((post#[implStatusIdx] = msiM /\
+              post#[implDirIdx].(snd) = msiI) \/
+             (post#[implStatusIdx] = msiS /\
+              post#[implDirIdx].(snd) = msiI))
+
+        | (c1pRs, msiDownRsS):
+            cost1 <-- oss@[child1Idx];
+            cost1#[implStatusIdx] = msiS /\             
+            msg_value (valOf eout) = VNat cost1#[implValueIdx]
+        | (c2pRs, msiDownRsS):
+            cost2 <-- oss@[child2Idx];
+            cost2#[implStatusIdx] = msiS /\
+            msg_value (valOf eout) = VNat cost2#[implValueIdx]
+
+        | (c1pRs, msiDownRsM):
+            cost1 <-- oss@[child1Idx];
+            cost1#[implStatusIdx] = msiI
+        | (c2pRs, msiDownRsM):
+            cost2 <-- oss@[child2Idx];
+            cost2#[implStatusIdx] = msiI
+        end.
+
+    Lemma msiSvMsgOutPred_good:
+      GoodMsgOutPred topo impl MsiSvMsgOutPred.
+    Proof.
+    Admitted.
+
+    Definition MsiSvLockPred (oidx: IdxT) (orq: ORq Msg): Prop :=
+      match case oidx on eq_nat_dec default True with
+      | child1Idx: True
+      | child2Idx: True
+      | parentIdx:
+          rqid <+- orq@[downRq];
+          ((rqid.(rqi_minds_rss) = [c2pRs] /\ rqid.(rqi_midx_rsb) = pc1) \/
+           (rqid.(rqi_minds_rss) = [c1pRs] /\ rqid.(rqi_midx_rsb) = pc2))
+      end.
+
+    Ltac disc_AtomicInv :=
+      repeat
+        match goal with
+        | [H: AtomicInv _ _ _ _ _ _ _ |- _] => red in H; dest
+        end.
+
+    Ltac disc_rule_custom ::=
+      try disc_footprints_ok;
+      try disc_AtomicInv.
+
+    Ltac atomic_cont_exfalso_bound :=
+      exfalso;
+      disc_rule_conds_ex;
+      repeat 
+        match goal with
+        | [H1: AtomicMsgOutsInv _ ?eouts _, H2: In _ ?eouts |- _] =>
+          red in H1; rewrite Forall_forall in H1;
+          specialize (H1 _ H2); simpl in H1
+        | [H: MsiSvMsgOutPred _ _ _ |- _] => red in H
+        | [H1: caseDec _ ?mii _ _ |- _] =>
+          match mii with
+          | miiOf (?midx, ?msg) =>
+            match goal with
+            | [H2: msg_id ?msg = ?mid |- _] =>
+              progress replace mii with (midx, mid) in H1
+                by (unfold miiOf; simpl; rewrite H2; reflexivity);
+              simpl in H1
+            end
+          end
+        end;
+      assumption.
+
+    Ltac atomic_init_exfalso_rq :=
+      exfalso;
+      disc_rule_conds_ex;
+      repeat
+        match goal with
+        | [H: _ = _ \/ _ |- _] =>
+          destruct H; [subst; try discriminate|auto]
+        end.
+
+    Ltac atomic_init_exfalso_rs_from_parent :=
+      exfalso;
+      repeat
+        (repeat match goal with
+                | [H: UpLockInvORq _ _ _ _ _ |- _] => red in H
+                | [H1: ?orq@[0] = Some _, H2: context[?orq@[0]] |- _] =>
+                  rewrite H1 in H2; simpl in H2
+                | [H: UpLockRsFromParent _ _ _ |- _] =>
+                  let rsFrom := fresh "rsFrom" in
+                  destruct H as [rsFrom [? ?]]
+                end;
+         disc_rule_conds_ex);
+      repeat
+        match goal with
+        | [H1: _ = ?rsFrom \/ _, H2: edgeDownTo _ _ = Some ?rsFrom |- _] =>
+          destruct H1; [subst; try discriminate|auto]
+        end.
+
+    Ltac atomic_init_exfalso_rs_to_parent :=
+      exfalso;
+      pose proof msiSv_impl_RqRsDTree;
+      repeat
+        (repeat match goal with
+                | [H: DownLockInvORq _ _ _ _ _ |- _] => red in H
+                | [H1: ?orq@[1] = Some _, H2: context[?orq@[1]] |- _] =>
+                  rewrite H1 in H2; simpl in H2
+                | [H: DownLockRssToParent _ _ _ |- _] => red in H
+                | [H: _ = rqi_minds_rss _ |- _] => apply eq_sym in H
+                end;
+         disc_rule_conds_ex);
+      repeat
+        match goal with
+        | [H1: _ = ?rsFrom \/ _, H2: rsEdgeUpFrom _ _ = Some ?rsFrom |- _] =>
+          destruct H1; [subst; try discriminate|auto]
+        end.
+
+    Ltac atomic_init_solve_AtomicMsgOutsInv :=
+      simpl; repeat constructor.
+
+    Ltac atomic_init_solve_AtomicLocksInv :=
+      red; intros; dest_in;
+      repeat (simpl; mred);
+      unfold miiOf; simpl;
+      repeat
+        match goal with
+        | [H: msg_id ?msg = _ |- context [msg_id ?msg] ] => rewrite H
+        | [H1: msg_id ?msg = _, H2: context [msg_id ?msg] |- _] =>
+          rewrite H1 in H2
+        | [H: ?orq@[?i] = Some _ |- context [?orq@[?i]] ] => rewrite H
+        | [H1: ?orq@[?i] = Some _, H2: context [?orq@[?i]] |- _] =>
+          rewrite H1 in H2
+        | [H: ?orq@[?i] = None |- context [?orq@[?i]] ] => rewrite H
+        | [H1: ?orq@[?i] = None, H2: context [?orq@[?i]] |- _] =>
+          rewrite H1 in H2
+        end;
+      repeat (red; simpl; mred; auto).
+
+    Local Ltac atomic_init_solve_AtomicInv :=
+      split; [atomic_init_solve_AtomicMsgOutsInv
+             |atomic_init_solve_AtomicLocksInv].
+
+    Lemma msiSv_impl_InvTrs_init:
+      forall st1,
+        Reachable (steps step_m) impl st1 ->
+        ImplStateInv st1 ->
+        forall oidx ridx ins outs st2,
+          SubList (idsOf ins) (sys_merqs impl) ->
+          step_m impl st1 (RlblInt oidx ridx ins outs) st2 ->
+          AtomicInv
+            MsiSvMsgOutPred MsiSvLockPred
+            ins st1 [RlblInt oidx ridx ins outs] outs st2 /\
+          ImplStateInv st2.
+    Proof.
+      intros.
+      inv_step.
+      pose proof (upLockInv_ok
+                    msiSv_impl_ORqsInit
+                    msiSv_impl_GoodRqRsSys
+                    msiSv_impl_RqRsDTree H) as Hulinv.
+      pose proof (downLockInv_ok
+                    msiSv_impl_ORqsInit
+                    msiSv_impl_GoodRqRsSys
+                    msiSv_impl_RqRsDTree
+                    msiSv_impl_GoodExtRssSys H) as Hdlinv.
+      good_locking_get obj.
+      dest_in.
+
+      (** List of [Rule]s:
+       * [childGetRqImm; childGetRqS; childGetRsS; childDownRqS; 
+       *  childSetRqImm; childSetRqM; childSetRsM; childDownRqM;
+       *  childEvictRqI; childEvictRsI] for [child1Idx] ++
+       * [childGetRqImm; childGetRqS; childGetRsS; childDownRqS; 
+       *  childSetRqImm; childSetRqM; childSetRsM; childDownRqM;
+       *  childEvictRqI; childEvictRsI] for [child2Idx] ++
+       * [parentGetRqImm; parentGetDownRqS; parentSetRqImm; parentSetDownRqM;
+       *  parentGetDownRsS; parentSetDownRsM;
+       *  parentEvictRqImmS; parentEvictRqImmLastS; parentEvictRqImmM] * 2
+       *)
+
+      3, 7, 10, 13, 17, 20: atomic_init_exfalso_rs_from_parent.
+      all: try (atomic_init_exfalso_rq; fail).
+
+      - (** [childGetRqImm] *)
+        disc_rule_conds_ex.
+        simpl; split; [atomic_init_solve_AtomicInv|].
+        replace (oss +[child1Idx <- pos]) with oss by meq.
+        replace (orqs +[child1Idx <- norq]) with orqs by meq.
+        assumption.
+
+      - (** [childGetRqS] *)
+        disc_rule_conds_ex.
+        simpl; split; [atomic_init_solve_AtomicInv|].
+        replace (oss +[child1Idx <- pos]) with oss by meq.
+        eapply implStateInv_orqs_weakened in H0; eauto.
+
+      - (** [childSetRqImm] *)
+        disc_rule_conds_ex.
+        simpl; split; [atomic_init_solve_AtomicInv|].
+        replace (orqs +[child1Idx <- norq]) with orqs by meq.
+        eapply implStateCoh_M_value_changed in H0; eauto.
+
+      - (** [childSetRqM] *)
+        disc_rule_conds_ex.
+        simpl; split; [atomic_init_solve_AtomicInv|].
+        replace (oss +[child1Idx <- pos]) with oss by meq.
+        eapply implStateInv_orqs_weakened in H0; eauto.
+
+      - (** [childEvictRqI] *)
+        disc_rule_conds_ex.
+        simpl; split; [atomic_init_solve_AtomicInv|].
+        replace (oss +[child1Idx <- pos]) with oss by meq.
+        eapply implStateInv_orqs_weakened in H0; eauto.
+
+      - (** [childGetRqImm] *)
+        disc_rule_conds_ex.
+        simpl; split; [atomic_init_solve_AtomicInv|].
+        replace (oss +[child2Idx <- pos]) with oss by meq.
+        replace (orqs +[child2Idx <- norq]) with orqs by meq.
+        assumption.
+
+      - (** [childGetRqS] *)
+        disc_rule_conds_ex.
+        simpl; split; [atomic_init_solve_AtomicInv|].
+        replace (oss +[child2Idx <- pos]) with oss by meq.
+        eapply implStateInv_orqs_weakened in H0; eauto.
+
+      - (** [childSetRqImm] *)
+        disc_rule_conds_ex.
+        simpl; split; [atomic_init_solve_AtomicInv|].
+        replace (orqs +[child2Idx <- norq]) with orqs by meq.
+        eapply implStateCoh_M_value_changed in H0; eauto.
+
+      - (** [childSetRqM] *)
+        disc_rule_conds_ex.
+        simpl; split; [atomic_init_solve_AtomicInv|].
+        replace (oss +[child2Idx <- pos]) with oss by meq.
+        eapply implStateInv_orqs_weakened in H0; eauto.
+
+      - (** [childEvictRqI] *)
+        disc_rule_conds_ex.
+        simpl; split; [atomic_init_solve_AtomicInv|].
+        replace (oss +[child2Idx <- pos]) with oss by meq.
+        eapply implStateInv_orqs_weakened in H0; eauto.
+    Qed.
+
+    Lemma miisOf_app:
+      forall miis1 miis2,
+        miisOf (miis1 ++ miis2) = miisOf miis1 ++ miisOf miis2.
+    Proof.
+      unfold miisOf; intros.
+      apply map_app.
+    Qed.
+
+    Ltac obj_visited_rsDown oidx :=
+      try match goal with
+          | [Ha: Atomic _ _ _ ?hst _ _ |- _] =>
+            assert (In oidx (oindsOf hst))
+              by (eapply extAtomic_rsDown_acceptor_visited; eauto;
+                  [exact msiSv_impl_ORqsInit
+                  |exact msiSv_impl_RqRsSys
+                  |econstructor; eassumption
+                  |red; auto])
+          end.
+
+    Ltac obj_visited_rsUp oidx ocidx :=
+      try match goal with
+          | [Ha: Atomic _ _ _ ?hst _ _ |- _] =>
+            assert (In parentIdx (oindsOf hst))
+              by (eapply extAtomic_rsUp_acceptor_visited
+                    with (cidx:= ocidx); eauto;
+                  [exact msiSv_impl_ORqsInit
+                  |exact msiSv_impl_RqRsSys
+                  |econstructor; eassumption
+                  |red; auto
+                  |reflexivity])
+          end.
+
+    Ltac disc_lock_preds_with Hl oidx :=
+      match type of Hl with
+      | AtomicLocksInv _ ?hst _ =>
+        match goal with
+        | [Hin: In oidx (oindsOf ?hst) |- _] =>
+          specialize (Hl _ Hin); simpl in Hl;
+          disc_rule_conds_ex; red in Hl; simpl in Hl
+        end
+      end.
+
+    Ltac disc_lock_preds oidx :=
+      match goal with
+      | [H: AtomicLocksInv _ _ _ |- _] =>
+        let Hl := fresh "H" in
+        pose proof H as Hl;
+        disc_lock_preds_with Hl oidx
+      end.
+
+    Ltac disc_mii_caseDec :=
+      match goal with
+      | [H1: caseDec _ ?mii _ _ |- _] =>
+        match mii with
+        | miiOf (?midx, ?msg) =>
+          match goal with
+          | [H2: msg_id ?msg = ?mid |- _] =>
+            progress replace mii with (midx, mid) in H1
+              by (unfold miiOf; simpl; rewrite H2; reflexivity);
+            simpl in H1
+          end
+        end
+      end.
+
+    Ltac disc_msg_preds_with Hl Hin :=
+      match type of Hl with
+      | AtomicMsgOutsInv _ ?eouts _ =>
+        red in Hl; rewrite Forall_forall in Hl;
+        specialize (Hl _ Hin); simpl in Hl;
+        red in Hl; disc_mii_caseDec
+      end.
+
+    Ltac disc_msg_preds Hin :=
+      match goal with
+      | [H: AtomicMsgOutsInv _ _ _ |- _] =>
+        let Hl := fresh "H" in
+        pose proof H as Hl;
+        disc_msg_preds_with Hl Hin
+      end.
+    
+    Ltac disc_minds_const :=
+      repeat
+        match goal with
+        | [H: rqEdgeUpFrom ?dtr ?oidx = Some ?midx |- _] =>
+          is_const dtr; is_const oidx; is_var midx; inv H
+        | [H: rsEdgeUpFrom ?dtr ?oidx = Some ?midx |- _] =>
+          is_const dtr; is_const oidx; is_var midx; inv H
+        | [H: edgeDownTo ?dtr ?oidx = Some ?midx |- _] =>
+          is_const dtr; is_const oidx; is_var midx; inv H
+        end.
+
+    Ltac disc_rule_custom ::=
+      try disc_footprints_ok;
+      try disc_msg_case;
+      try disc_AtomicInv;
+      try disc_msi;
+      try disc_minds_const.
+
+    Lemma msiSv_impl_InvTrs: InvTrs impl ImplStateInv.
+    Proof.
+      eapply inv_atomic_InvTrs;
+        [red; intros; eapply msiSv_impl_InvTrs_ext_in; eauto
+        |red; intros; eapply msiSv_impl_InvTrs_ext_out; eauto
+        |].
+      instantiate (1:= AtomicInv MsiSvMsgOutPred MsiSvLockPred).
+      red; intros.
+      destruct H1.
+      generalize dependent ist2.
+      induction H3; simpl; intros; subst;
+        [inv_steps; apply msiSv_impl_InvTrs_init; auto|].
+
+      inv_steps.
+      pose proof (footprints_ok
+                    msiSv_impl_ORqsInit
+                    msiSv_impl_GoodRqRsSys
+                    (reachable_steps H H9))
+        as Hftinv.
+      specialize (IHAtomic H1 _ H9); dest.
+      pose proof (upLockInv_ok
+                    msiSv_impl_ORqsInit
+                    msiSv_impl_GoodRqRsSys
+                    msiSv_impl_RqRsDTree (reachable_steps H H9)) as Hulinv.
+      pose proof (downLockInv_ok
+                    msiSv_impl_ORqsInit
+                    msiSv_impl_GoodRqRsSys
+                    msiSv_impl_RqRsDTree
+                    msiSv_impl_GoodExtRssSys (reachable_steps H H9)) as Hdlinv.
+      inv_step; dest_in.
+
+      (** child1 *)
+
+      - atomic_cont_exfalso_bound.
+      - atomic_cont_exfalso_bound.
+
+      - (** [childGetRsS] *)
+        disc_rule_conds_ex.
+        good_footprint_get child1Idx.
+        disc_rule_conds_ex.
+
+        (* discharge lock predicates *)
+        obj_visited_rsDown child1Idx.
+        disc_lock_preds child1Idx.
+        disc_rule_conds_ex.
+
+        (* discharge message predicates *)
+        disc_msg_preds H4.
+        disc_rule_conds_ex.
+
+        (* generate hints for leaves (L1 caches) *)
+        pose proof (parentIdxOf_child_indsOf _ _ H8).
+        dest_in; try discriminate; simpl in *.
+        cbn in H24; inv H24.
+
+        (* construction *)
+        split.
+        + split.
+          * apply Forall_app.
+            { apply forall_removeOnce.
+              eapply atomic_rsDown_preserves_msg_out_preds; eauto;
+                [exact msiSv_impl_ORqsInit
+                |exact msiSv_impl_RqRsSys
+                |red; auto
+                |exact msiSvMsgOutPred_good].
+            }
+            { repeat (constructor; simpl). }
+          * red; simpl; intros.
+            icase oidx.
+            { repeat (simpl; red; mred). }
+            { mred; apply H7; auto. }
+        + red in H6; red; simpl in *; mred; simpl.
+          destruct (oss@[child2Idx]) as [cost2|]; simpl in *; [|auto].
+          destruct (orqs@[child2Idx]) as [corq2|]; simpl in *; [|auto].
+          destruct H6 as [[cv ?] ?].
+          red in H6; dest.
+          split.
+          * exists val0.
+            red; repeat ssplit.
+            { solve_rule_conds_ex. }
+            { solve_rule_conds_ex. }
+            { solve_rule_conds_ex.
+              unfold msiM, msiS, msiI in *; lia.
+            }
+            { solve_rule_conds_ex.
+              unfold msiM, msiS, msiI in *; lia.
+            }
+          * solve_rule_conds_ex.
+
+      - (** [childDownRqS] *)
+        disc_rule_conds_ex.
+
+        (* construction *)
+        split.
+        + split.
+          * apply Forall_app.
+            { apply forall_removeOnce.
+              eapply atomic_rqDown_preserves_msg_out_preds; eauto;
+                [exact msiSv_impl_ORqsInit
+                |exact msiSv_impl_RqRsSys
+                |red; auto
+                |exact msiSvMsgOutPred_good].
+            }
+            { repeat (constructor; simpl).
+              red; simpl.
+              mred; simpl; auto.
+            }
+          * red; simpl; intros.
+            icase oidx.
+            { mred. }
+            { mred; apply H7; auto. }
+        + red in H6; red; simpl in *; mred; simpl.
+          destruct (oss@[parentIdx]) as [post|] eqn:Hpost; simpl in *; [|auto].
+          destruct (oss@[child2Idx]) as [cost2|] eqn:Hcost2; simpl in *; [|auto].
+          destruct (orqs@[parentIdx]) as [porq|] eqn:Hporq; simpl in *; [|auto].
+          destruct (orqs@[child2Idx]) as [corq2|] eqn:Hcorq2; simpl in *; [|auto].
+          destruct H6 as [[cv ?] ?].
+          red in H6; dest.
+          split.
+          * exists cv.
+            red; repeat ssplit.
+            { solve_rule_conds_ex. }
+            { solve_rule_conds_ex. }
+            { solve_rule_conds_ex. }
+            { solve_rule_conds_ex.
+              unfold msiM, msiS, msiI in *; lia.
+            }
+          * disc_rule_conds_ex.
+            exfalso.
+            assert (In parent (sys_objs impl)) by (simpl; tauto).
+            good_locking_get parent.
+            clear H24.
+            eapply downLockInvORq_down_rqsQ_length_one_locked
+              with (cidx:= child1Idx) in H27; eauto;
+              [|reflexivity
+               |eapply rqsQ_length_ge_one; [eauto|apply FirstMP_InMP; assumption]].
+            destruct H27 as [rqid [? [? [rsUp ?]]]]; dest.
+            disc_rule_conds_ex.
+
+      - atomic_cont_exfalso_bound.
+      - atomic_cont_exfalso_bound.
+      - (** [childSetRsM] *)
+        disc_rule_conds_ex.
+        good_footprint_get child1Idx.
+        disc_rule_conds_ex.
+
+        (* discharge lock predicates *)
+        obj_visited_rsDown child1Idx.
+        disc_lock_preds child1Idx.
+        disc_rule_conds_ex.
+
+        (* discharge message predicates *)
+        disc_msg_preds H4.
+        disc_rule_conds_ex.
+
+        (* generate hints for leaves (L1 caches) *)
+        pose proof (parentIdxOf_child_indsOf _ _ H8).
+        dest_in; try discriminate; simpl in *.
+        cbn in H24; inv H24.
+
+        (* construction *)
+        split.
+        + split.
+          * apply Forall_app.
+            { apply forall_removeOnce.
+              eapply atomic_rsDown_preserves_msg_out_preds; eauto;
+                [exact msiSv_impl_ORqsInit
+                |exact msiSv_impl_RqRsSys
+                |red; auto
+                |exact msiSvMsgOutPred_good].
+            }
+            { repeat (constructor; simpl). }
+          * red; simpl; intros.
+            icase oidx.
+            { repeat (simpl; red; mred). }
+            { mred; apply H7; auto. }
+        + red in H6; red; simpl in *; mred; simpl.
+          destruct (oss@[child2Idx]) as [cost2|]; simpl in *; [|auto].
+          destruct (orqs@[child2Idx]) as [corq2|]; simpl in *; [|auto].
+          destruct H6 as [[cv ?] ?].
+          red in H6; dest.
+          split.
+          * exists n.
+            red; repeat ssplit.
+            { solve_rule_conds_ex.
+              destruct H6 as [|[|]]; try (exfalso; dest; discriminate).
+              right; right; solve_rule_conds_ex.
+            }
+            { solve_rule_conds_ex. }
+            { solve_rule_conds_ex.
+              unfold msiM, msiS, msiI in *; lia.
+            }
+            { solve_rule_conds_ex.
+              { unfold msiM, msiS, msiI in *; lia. }
+              { unfold msiM, msiS, msiI in *; lia. }
+            }
+          * solve_rule_conds_ex.
+
+      - (** [childDownRqM] *)
+        disc_rule_conds_ex.
+
+        (* construction *)
+        split.
+        + split.
+          * apply Forall_app.
+            { apply forall_removeOnce.
+              eapply atomic_rqDown_preserves_msg_out_preds; eauto;
+                [exact msiSv_impl_ORqsInit
+                |exact msiSv_impl_RqRsSys
+                |red; auto
+                |exact msiSvMsgOutPred_good].
+            }
+            { repeat (constructor; simpl).
+              red; simpl.
+              mred; simpl; auto.
+            }
+          * red; simpl; intros.
+            icase oidx.
+            { mred. }
+            { mred; apply H7; auto. }
+        + red in H6; red; simpl in *; mred; simpl.
+          destruct (oss@[parentIdx]) as [post|] eqn:Hpost; simpl in *; [|auto].
+          destruct (oss@[child2Idx]) as [cost2|] eqn:Hcost2; simpl in *; [|auto].
+          destruct (orqs@[parentIdx]) as [porq|] eqn:Hporq; simpl in *; [|auto].
+          destruct (orqs@[child2Idx]) as [corq2|] eqn:Hcorq2; simpl in *; [|auto].
+          destruct H6 as [[cv ?] ?].
+          red in H6; dest.
+          split.
+          * exists cv.
+            red; repeat ssplit.
+            { solve_rule_conds_ex. }
+            { solve_rule_conds_ex. }
+            { solve_rule_conds_ex. }
+            { solve_rule_conds_ex. }
+          * disc_rule_conds_ex.
+            exfalso.
+            assert (In parent (sys_objs impl)) by (simpl; tauto).
+            good_locking_get parent.
+            clear H24.
+            eapply downLockInvORq_down_rqsQ_length_one_locked
+              with (cidx:= child1Idx) in H27; eauto;
+              [|reflexivity
+               |eapply rqsQ_length_ge_one; [eauto|apply FirstMP_InMP; assumption]].
+            destruct H27 as [rqid [? [? [rsUp ?]]]]; dest.
+            disc_rule_conds_ex.
+
+      - atomic_cont_exfalso_bound.
+      - (** [childEvictRsI] *)
+        disc_rule_conds_ex.
+        good_footprint_get child1Idx.
+        disc_rule_conds_ex.
+
+        (* discharge lock predicates *)
+        obj_visited_rsDown child1Idx.
+        disc_lock_preds child1Idx.
+        disc_rule_conds_ex.
+
+        (* discharge message predicates *)
+        disc_msg_preds H4.
+        disc_rule_conds_ex.
+
+        (* generate hints for leaves (L1 caches) *)
+        pose proof (parentIdxOf_child_indsOf _ _ H8).
+        dest_in; try discriminate; simpl in *.
+        cbn in H22; inv H22.
+
+        (* construction *)
+        split.
+        + split.
+          * apply Forall_app.
+            { apply forall_removeOnce.
+              eapply atomic_rsDown_preserves_msg_out_preds; eauto;
+                [exact msiSv_impl_ORqsInit
+                |exact msiSv_impl_RqRsSys
+                |red; auto
+                |exact msiSvMsgOutPred_good].
+            }
+            { repeat (constructor; simpl). }
+          * red; simpl; intros.
+            icase oidx.
+            { repeat (simpl; red; mred). }
+            { mred; apply H7; auto. }
+        + red in H6; red; simpl in *; mred; simpl.
+          rename porq into orq.
+          destruct (oss@[child2Idx]) as [cost2|]; simpl in *; [|auto].
+          destruct (orqs@[parentIdx]) as [porq|]; simpl in *; [|auto].
+          destruct (orqs@[child2Idx]) as [corq2|]; simpl in *; [|auto].
+          destruct H6 as [[cv ?] ?].
+          red in H6; dest.
+          split.
+          * exists cv.
+            clear H22.
+            red; repeat ssplit.
+            { solve_rule_conds_ex. }
+            { solve_rule_conds_ex.
+              unfold msiM, msiS, msiI in *; lia.
+            }
+            { solve_rule_conds_ex. }
+            { solve_rule_conds_ex. }
+          * destruct H24.
+            { solve_rule_conds_ex. }
+            { solve_rule_conds_ex. }
+
+      (** child2 *)
+      - atomic_cont_exfalso_bound.
+      - atomic_cont_exfalso_bound.
+
+      - (** [childGetRsS] *)
+        disc_rule_conds_ex.
+        good_footprint_get child2Idx.
+        disc_rule_conds_ex.
+
+        (* discharge lock predicates *)
+        obj_visited_rsDown child2Idx.
+        disc_lock_preds child2Idx.
+        disc_rule_conds_ex.
+
+        (* discharge message predicates *)
+        disc_msg_preds H4.
+        disc_rule_conds_ex.
+
+        (* generate hints for leaves (L1 caches) *)
+        pose proof (parentIdxOf_child_indsOf _ _ H8).
+        dest_in; try discriminate; simpl in *.
+        cbn in H24; inv H24.
+
+        (* construction *)
+        split.
+        + split.
+          * apply Forall_app.
+            { apply forall_removeOnce.
+              eapply atomic_rsDown_preserves_msg_out_preds; eauto;
+                [exact msiSv_impl_ORqsInit
+                |exact msiSv_impl_RqRsSys
+                |red; auto
+                |exact msiSvMsgOutPred_good].
+            }
+            { repeat (constructor; simpl). }
+          * red; simpl; intros.
+            icase oidx.
+            { repeat (simpl; red; mred). }
+            { mred; apply H7; auto. }
+        + red in H6; red; simpl in *; mred; simpl.
+          destruct (oss@[child1Idx]) as [cost1|]; simpl in *; [|auto].
+          destruct (orqs@[child1Idx]) as [corq1|]; simpl in *; [|auto].
+          destruct H6 as [[cv ?] ?].
+          red in H6; dest.
+          split.
+          * exists val0.
+            red; repeat ssplit.
+            { solve_rule_conds_ex. }
+            { solve_rule_conds_ex.
+              unfold msiM, msiS, msiI in *; lia.
+            }
+            { solve_rule_conds_ex. }
+            { solve_rule_conds_ex.
+              unfold msiM, msiS, msiI in *; lia.
+            }
+          * solve_rule_conds_ex.
+
+      - (** [childDownRqS] *)
+        disc_rule_conds_ex.
+
+        (* construction *)
+        split.
+        + split.
+          * apply Forall_app.
+            { apply forall_removeOnce.
+              eapply atomic_rqDown_preserves_msg_out_preds; eauto;
+                [exact msiSv_impl_ORqsInit
+                |exact msiSv_impl_RqRsSys
+                |red; auto
+                |exact msiSvMsgOutPred_good].
+            }
+            { repeat (constructor; simpl).
+              red; simpl.
+              mred; simpl; auto.
+            }
+          * red; simpl; intros.
+            icase oidx.
+            { mred. }
+            { mred; apply H7; auto. }
+        + red in H6; red; simpl in *; mred; simpl.
+          destruct (oss@[parentIdx]) as [post|] eqn:Hpost; simpl in *; [|auto].
+          destruct (oss@[child1Idx]) as [cost1|] eqn:Hcost1; simpl in *; [|auto].
+          destruct (orqs@[parentIdx]) as [porq|] eqn:Hporq; simpl in *; [|auto].
+          destruct (orqs@[child1Idx]) as [corq1|] eqn:Hcorq1; simpl in *; [|auto].
+          destruct H6 as [[cv ?] ?].
+          red in H6; dest.
+          split.
+          * exists cv.
+            red; repeat ssplit.
+            { solve_rule_conds_ex. }
+            { solve_rule_conds_ex. }
+            { solve_rule_conds_ex. }
+            { solve_rule_conds_ex.
+              unfold msiM, msiS, msiI in *; lia.
+            }
+          * disc_rule_conds_ex.
+            exfalso.
+            assert (In parent (sys_objs impl)) by (simpl; tauto).
+            good_locking_get parent.
+            clear H24.
+            eapply downLockInvORq_down_rqsQ_length_one_locked
+              with (cidx:= child2Idx) in H27; eauto;
+              [|reflexivity
+               |eapply rqsQ_length_ge_one; [eauto|apply FirstMP_InMP; assumption]].
+            destruct H27 as [rqid [? [? [rsUp ?]]]]; dest.
+            disc_rule_conds_ex.
+        
+      - atomic_cont_exfalso_bound.
+      - atomic_cont_exfalso_bound.
+      - (** [childSetRsM] *)
+        disc_rule_conds_ex.
+        good_footprint_get child2Idx.
+        disc_rule_conds_ex.
+
+        (* discharge lock predicates *)
+        obj_visited_rsDown child2Idx.
+        disc_lock_preds child2Idx.
+        disc_rule_conds_ex.
+
+        (* discharge message predicates *)
+        disc_msg_preds H4.
+        disc_rule_conds_ex.
+
+        (* generate hints for leaves (L1 caches) *)
+        pose proof (parentIdxOf_child_indsOf _ _ H8).
+        dest_in; try discriminate; simpl in *.
+        cbn in H24; inv H24.
+
+        (* construction *)
+        split.
+        + split.
+          * apply Forall_app.
+            { apply forall_removeOnce.
+              eapply atomic_rsDown_preserves_msg_out_preds; eauto;
+                [exact msiSv_impl_ORqsInit
+                |exact msiSv_impl_RqRsSys
+                |red; auto
+                |exact msiSvMsgOutPred_good].
+            }
+            { repeat (constructor; simpl). }
+          * red; simpl; intros.
+            icase oidx.
+            { repeat (simpl; red; mred). }
+            { mred; apply H7; auto. }
+        + red in H6; red; simpl in *; mred; simpl.
+          destruct (oss@[child1Idx]) as [cost1|]; simpl in *; [|auto].
+          destruct (orqs@[child1Idx]) as [corq1|]; simpl in *; [|auto].
+          destruct H6 as [[cv ?] ?].
+          red in H6; dest.
+          split.
+          * exists n.
+            red; repeat ssplit.
+            { solve_rule_conds_ex.
+              destruct H6 as [|[|]]; try (exfalso; dest; discriminate).
+              right; right; solve_rule_conds_ex.
+            }
+            { solve_rule_conds_ex.
+              unfold msiM, msiS, msiI in *; lia.
+            }
+            { solve_rule_conds_ex. }
+            { solve_rule_conds_ex.
+              { unfold msiM, msiS, msiI in *; lia. }
+              { unfold msiM, msiS, msiI in *; lia. }
+            }
+          * solve_rule_conds_ex.
+          
+      - (** [childDownRqM] *)
+        disc_rule_conds_ex.
+
+        (* construction *)
+        split.
+        + split.
+          * apply Forall_app.
+            { apply forall_removeOnce.
+              eapply atomic_rqDown_preserves_msg_out_preds; eauto;
+                [exact msiSv_impl_ORqsInit
+                |exact msiSv_impl_RqRsSys
+                |red; auto
+                |exact msiSvMsgOutPred_good].
+            }
+            { repeat (constructor; simpl).
+              red; simpl.
+              mred; simpl; auto.
+            }
+          * red; simpl; intros.
+            icase oidx.
+            { mred. }
+            { mred; apply H7; auto. }
+        + red in H6; red; simpl in *; mred; simpl.
+          destruct (oss@[parentIdx]) as [post|] eqn:Hpost; simpl in *; [|auto].
+          destruct (oss@[child1Idx]) as [cost1|] eqn:Hcost1; simpl in *; [|auto].
+          destruct (orqs@[parentIdx]) as [porq|] eqn:Hporq; simpl in *; [|auto].
+          destruct (orqs@[child1Idx]) as [corq1|] eqn:Hcorq1; simpl in *; [|auto].
+          destruct H6 as [[cv ?] ?].
+          red in H6; dest.
+          split.
+          * exists cv.
+            red; repeat ssplit.
+            { solve_rule_conds_ex. }
+            { solve_rule_conds_ex. }
+            { solve_rule_conds_ex. }
+            { solve_rule_conds_ex. }
+          * disc_rule_conds_ex.
+            exfalso.
+            assert (In parent (sys_objs impl)) by (simpl; tauto).
+            good_locking_get parent.
+            clear H24.
+            eapply downLockInvORq_down_rqsQ_length_one_locked
+              with (cidx:= child2Idx) in H27; eauto;
+              [|reflexivity
+               |eapply rqsQ_length_ge_one; [eauto|apply FirstMP_InMP; assumption]].
+            destruct H27 as [rqid [? [? [rsUp ?]]]]; dest.
+            disc_rule_conds_ex.
+
+      - atomic_cont_exfalso_bound.
+      - (** [childEvictRsI] *)
+        disc_rule_conds_ex.
+        good_footprint_get child2Idx.
+        disc_rule_conds_ex.
+
+        (* discharge lock predicates *)
+        obj_visited_rsDown child2Idx.
+        disc_lock_preds child2Idx.
+        disc_rule_conds_ex.
+
+        (* discharge message predicates *)
+        disc_msg_preds H4.
+        disc_rule_conds_ex.
+
+        (* generate hints for leaves (L1 caches) *)
+        pose proof (parentIdxOf_child_indsOf _ _ H8).
+        dest_in; try discriminate; simpl in *.
+        cbn in H22; inv H22.
+
+        (* construction *)
+        split.
+        + split.
+          * apply Forall_app.
+            { apply forall_removeOnce.
+              eapply atomic_rsDown_preserves_msg_out_preds; eauto;
+                [exact msiSv_impl_ORqsInit
+                |exact msiSv_impl_RqRsSys
+                |red; auto
+                |exact msiSvMsgOutPred_good].
+            }
+            { repeat (constructor; simpl). }
+          * red; simpl; intros.
+            icase oidx.
+            { repeat (simpl; red; mred). }
+            { mred; apply H7; auto. }
+        + red in H6; red; simpl in *; mred; simpl.
+          rename porq into orq.
+          destruct (oss@[child1Idx]) as [cost1|]; simpl in *; [|auto].
+          destruct (orqs@[parentIdx]) as [porq|]; simpl in *; [|auto].
+          destruct (orqs@[child1Idx]) as [corq1|]; simpl in *; [|auto].
+          destruct H6 as [[cv ?] ?].
+          red in H6; dest.
+          split.
+          * exists cv.
+            red; repeat ssplit.
+            { solve_rule_conds_ex. }
+            { solve_rule_conds_ex. }
+            { solve_rule_conds_ex.
+              unfold msiM, msiS, msiI in *; lia.
+            }
+            { solve_rule_conds_ex. }
+          * destruct H24.
+            { solve_rule_conds_ex. }
+            { solve_rule_conds_ex. }
+
+      (** parent(child1) *)
+
+      - (** [parentGetRqImm] *)
+        disc_rule_conds_ex.
+
+        split.
+        + split.
+          * apply Forall_app.
+            { apply forall_removeOnce.
+              eapply atomic_rqUp_preserves_msg_out_preds with (oidx:= child1Idx);
+                [exact msiSv_impl_ORqsInit
+                |exact msiSv_impl_RqRsSys|..]; eauto.
+              { intro; dest_in; discriminate. }
+              { red; auto. }
+              { exact msiSvMsgOutPred_good. }
+            }
+            { repeat (constructor; simpl).
+              red; repeat (simpl; mred).
+            }
+          * red; simpl; intros.
+            icase oidx.
+            { repeat (simpl; red; mred). }
+            { mred; apply H7; auto. }
+        + red in H6; red; simpl in *; mred; simpl.
+          destruct (oss@[child1Idx]) as [cost1|] eqn:Hcost1; simpl in *; [|auto].
+          destruct (oss@[child2Idx]) as [cost2|] eqn:Hcost2; simpl in *; [|auto].
+          destruct (orqs@[child1Idx]) as [corq1|] eqn:Hcorq1; simpl in *; [|auto].
+          destruct (orqs@[child2Idx]) as [corq2|] eqn:Hcorq2; simpl in *; [|auto].
+          destruct H6 as [[cv ?] ?].
+          red in H6; dest.
+          split.
+          * exists cv.
+            clear H8.
+            red; repeat ssplit.
+            { solve_rule_conds_ex.
+              right; left.
+              destruct H6 as [|[|]].
+              { solve_rule_conds_ex.
+                unfold msiM, msiS, msiI in *; lia.
+              }
+              { solve_rule_conds_ex. }
+              { unfold msiM, msiS, msiI in *; lia. }
+            }
+            { solve_rule_conds_ex. }
+            { solve_rule_conds_ex. }
+            { solve_rule_conds_ex. }
+          * disc_rule_conds_ex.
+            assert (In (child child1Idx ec1 ce1 c1pRq c1pRs pc1) (sys_objs impl))
+              by (simpl; tauto).
+            good_locking_get (child child1Idx ec1 ce1 c1pRq c1pRs pc1).
+            clear H24.
+            eapply upLockInvORq_rqUp_length_one_locked in H26; try reflexivity;
+              [|eapply findQ_length_ge_one; apply FirstMP_InMP; eassumption].
+            solve_rule_conds_ex.
+
+      - (** [parentGetDownRqS] *)
+        disc_rule_conds_ex.
+
+        split.
+        + split.
+          * apply Forall_app.
+            { apply forall_removeOnce.
+              eapply atomic_rqUp_preserves_msg_out_preds with (oidx:= child1Idx);
+                [exact msiSv_impl_ORqsInit
+                |exact msiSv_impl_RqRsSys|..]; eauto.
+              { intro; dest_in; discriminate. }
+              { red; auto. }
+              { exact msiSvMsgOutPred_good. }
+            }
+            { repeat (constructor; simpl). }
+          * red; simpl; intros.
+            icase oidx.
+            { repeat (simpl; red; mred).
+              simpl; left; auto.
+            }
+            { mred; apply H7; auto. }
+        + red in H6; red; simpl in *; mred; simpl.
+          destruct (oss@[child1Idx]) as [cost1|]; simpl in *; [|auto].
+          destruct (oss@[child2Idx]) as [cost2|]; simpl in *; [|auto].
+          destruct (orqs@[child1Idx]) as [corq1|]; simpl in *; [|auto].
+          destruct (orqs@[child2Idx]) as [corq2|]; simpl in *; [|auto].
+          destruct H6 as [[cv ?] ?].
+          red in H6; dest.
+          split.
+          * exists cv.
+            clear H8.
+            red; repeat ssplit.
+            { solve_rule_conds_ex. }
+            { solve_rule_conds_ex. }
+            { solve_rule_conds_ex. }
+            { solve_rule_conds_ex. }
+          * solve_rule_conds_ex.
+
+      - (** [parentSetRqImm] *)
+        disc_rule_conds_ex.
+
+        split.
+        + split.
+          * apply Forall_app.
+            { apply forall_removeOnce.
+              eapply atomic_rqUp_preserves_msg_out_preds with (oidx:= child1Idx);
+                [exact msiSv_impl_ORqsInit
+                |exact msiSv_impl_RqRsSys|..]; eauto.
+              { intro; dest_in; discriminate. }
+              { red; auto. }
+              { exact msiSvMsgOutPred_good. }
+            }
+            { repeat (constructor; simpl).
+              red; repeat (simpl; mred).
+            }
+          * red; simpl; intros.
+            icase oidx.
+            { repeat (simpl; red; mred). }
+            { mred; apply H7; auto. }
+        + red in H6; red; simpl in *; mred; simpl.
+          destruct (oss@[child1Idx]) as [cost1|] eqn:Hcost1; simpl in *; [|auto].
+          destruct (oss@[child2Idx]) as [cost2|] eqn:Hcost2; simpl in *; [|auto].
+          destruct (orqs@[child1Idx]) as [corq1|] eqn:Hcorq1; simpl in *; [|auto].
+          destruct (orqs@[child2Idx]) as [corq2|] eqn:Hcorq2; simpl in *; [|auto].
+          destruct H6 as [[cv ?] ?].
+          red in H6; dest.
+          unfold getDir in H14; simpl in H14.
+          split.
+          * exists cv.
+            red; repeat ssplit.
+            { solve_rule_conds_ex. }
+            { solve_rule_conds_ex. }
+            { solve_rule_conds_ex. }
+            { solve_rule_conds_ex. }
+          * disc_rule_conds_ex.
+            assert (In (child child1Idx ec1 ce1 c1pRq c1pRs pc1) (sys_objs impl))
+              by (simpl; tauto).
+            good_locking_get (child child1Idx ec1 ce1 c1pRq c1pRs pc1).
+            clear H24.
+            eapply upLockInvORq_rqUp_length_one_locked in H26; try reflexivity;
+              [|eapply findQ_length_ge_one; apply FirstMP_InMP; eassumption].
+            solve_rule_conds_ex.
+
+      - (** [parentSetDownRqM] *)
+        disc_rule_conds_ex.
+
+        split.
+        + split.
+          * apply Forall_app.
+            { apply forall_removeOnce.
+              eapply atomic_rqUp_preserves_msg_out_preds with (oidx:= child1Idx);
+                [exact msiSv_impl_ORqsInit
+                |exact msiSv_impl_RqRsSys|..]; eauto.
+              { intro; dest_in; discriminate. }
+              { red; auto. }
+              { exact msiSvMsgOutPred_good. }
+            }
+            { repeat (constructor; simpl). }
+          * red; simpl; intros.
+            icase oidx.
+            { repeat (simpl; red; mred).
+              simpl; left; auto.
+            }
+            { mred; apply H7; auto. }
+        + red in H6; red; simpl in *; mred; simpl.
+          destruct (oss@[child1Idx]) as [cost1|]; simpl in *; [|auto].
+          destruct (oss@[child2Idx]) as [cost2|]; simpl in *; [|auto].
+          destruct (orqs@[child1Idx]) as [corq1|]; simpl in *; [|auto].
+          destruct (orqs@[child2Idx]) as [corq2|]; simpl in *; [|auto].
+          destruct H6 as [[cv ?] ?].
+          red in H6; dest.
+          split.
+          * exists cv.
+            clear H8.
+            red; repeat ssplit.
+            { solve_rule_conds_ex. }
+            { solve_rule_conds_ex. }
+            { solve_rule_conds_ex. }
+            { solve_rule_conds_ex. }
+          * solve_rule_conds_ex.
+
+      - (** [parentGetDownRsS] *)
+        disc_rule_conds_ex.
+
+        obj_visited_rsUp parentIdx child2Idx.
+        disc_lock_preds parentIdx.
+        disc_rule_conds_ex.
+        destruct H11; dest; [|discriminate].
+        clear H11.
+        disc_rule_conds_ex.
+
+        (* discharge message predicates *)
+        disc_msg_preds H4.
+        disc_rule_conds_ex.
+        
+        split.
+        + split.
+          * apply Forall_app.
+            { apply forall_removeOnce.
+              eapply atomic_rsUps_preserves_msg_out_preds
+                with (rsUps:= [(c2pRs, rmsg)]); eauto.
+              { exact msiSv_impl_ORqsInit. }
+              { exact msiSv_impl_RqRsSys. }
+              { repeat constructor; intro; dest_in. }
+              { apply SubList_cons; [|apply SubList_nil].
+                assumption.
+              }
+              { instantiate (1:= fun _ => True).
+                instantiate (1:= [pc2]).
+                repeat split.
+                { discriminate. }
+                { repeat constructor.
+                  simpl; exists child2Idx.
+                  repeat split.
+                }
+              }
+              { exact msiSvMsgOutPred_good. }
+            }
+            { repeat (constructor; simpl).
+              red; simpl.
+              solve_rule_conds_ex.
+            }
+          * red; simpl; intros.
+            icase oidx.
+            { repeat (simpl; red; mred). }
+            { mred; apply H7; auto. }
+        + red in H6; red; simpl in *; mred; simpl.
+          destruct (oss@[child1Idx]) as [cost1|] eqn:Hcost1; simpl in *; [|auto].
+          destruct (orqs@[child1Idx]) as [corq1|] eqn:Hcorq1; simpl in *; [|auto].
+          destruct (orqs@[child2Idx]) as [corq2|] eqn:Hcorq2; simpl in *; [|auto].
+          destruct H6 as [[cv ?] ?].
+          red in H6; dest.
+
+          assert (In (child child1Idx ec1 ce1 c1pRq c1pRs pc1) (sys_objs impl))
+            by (simpl; tauto).
+          good_locking_get (child child1Idx ec1 ce1 c1pRq c1pRs pc1).
+          clear H24.
+          eapply upLockInvORq_parent_locked_locked in H26; try reflexivity;
+            [|red; repeat (simpl; mred); eauto]; dest.
+          
+          split.
+          * exists val0.
+            clear H11.
+            red; repeat ssplit.
+            { solve_rule_conds_ex.
+              right; left; auto.
+            }
+            { solve_rule_conds_ex. }
+            { solve_rule_conds_ex. }
+            { solve_rule_conds_ex. }
+          * solve_rule_conds_ex.
+
+      - (** [parentSetDownRsM] *)
+        disc_rule_conds_ex.
+
+        obj_visited_rsUp parentIdx child2Idx.
+        disc_lock_preds parentIdx.
+        disc_rule_conds_ex.
+        destruct H11; dest; [|discriminate].
+        clear H11.
+        disc_rule_conds_ex.
+
+        (* discharge message predicates *)
+        disc_msg_preds H4.
+        disc_rule_conds_ex.
+        
+        split.
+        + split.
+          * apply Forall_app.
+            { apply forall_removeOnce.
+              eapply atomic_rsUps_preserves_msg_out_preds
+                with (rsUps:= [(c2pRs, rmsg)]); eauto.
+              { exact msiSv_impl_ORqsInit. }
+              { exact msiSv_impl_RqRsSys. }
+              { repeat constructor; intro; dest_in. }
+              { apply SubList_cons; [|apply SubList_nil].
+                assumption.
+              }
+              { instantiate (1:= fun _ => True).
+                instantiate (1:= [pc2]).
+                repeat split.
+                { discriminate. }
+                { repeat constructor.
+                  simpl; exists child2Idx.
+                  repeat split.
+                }
+              }
+              { exact msiSvMsgOutPred_good. }
+            }
+            { repeat (constructor; simpl).
+              red; simpl.
+              solve_rule_conds_ex.
+            }
+          * red; simpl; intros.
+            icase oidx.
+            { repeat (simpl; red; mred). }
+            { mred; apply H7; auto. }
+        + red in H6; red; simpl in *; mred; simpl.
+          destruct (oss@[child1Idx]) as [cost1|] eqn:Hcost1; simpl in *; [|auto].
+          destruct (orqs@[child1Idx]) as [corq1|] eqn:Hcorq1; simpl in *; [|auto].
+          destruct (orqs@[child2Idx]) as [corq2|] eqn:Hcorq2; simpl in *; [|auto].
+          destruct H6 as [[cv ?] ?].
+          red in H6; dest.
+
+          assert (In (child child1Idx ec1 ce1 c1pRq c1pRs pc1) (sys_objs impl))
+            by (simpl; tauto).
+          good_locking_get (child child1Idx ec1 ce1 c1pRq c1pRs pc1).
+          clear H24.
+          eapply upLockInvORq_parent_locked_locked in H26; try reflexivity;
+            [|red; repeat (simpl; mred); eauto]; dest.
+
+          split.
+          * exists val0.
+            clear H11.
+            red; repeat ssplit.
+            { solve_rule_conds_ex. }
+            { solve_rule_conds_ex. }
+            { solve_rule_conds_ex. }
+            { solve_rule_conds_ex. }
+          * solve_rule_conds_ex.
+
+      - (** [parentEvictRqImmS] *)
+        disc_rule_conds_ex.
+
+        split.
+        + split.
+          * apply Forall_app.
+            { apply forall_removeOnce.
+              eapply atomic_rqUp_preserves_msg_out_preds with (oidx:= child1Idx);
+                [exact msiSv_impl_ORqsInit
+                |exact msiSv_impl_RqRsSys|..]; eauto.
+              { intro; dest_in; discriminate. }
+              { red; auto. }
+              { exact msiSvMsgOutPred_good. }
+            }
+            { repeat (constructor; simpl).
+              red; repeat (simpl; mred).
+              red in H6; simpl in H6.
+              unfold getDir in *; simpl in *.
+              disc_rule_conds_ex.
+              destruct H6 as [|[|]]; dest.
+              { exfalso; solve_rule_conds_ex. }
+              { subst; auto. }
+              { exfalso; destruct H26; solve_rule_conds_ex. }
+            }
+          * red; simpl; intros.
+            icase oidx.
+            { repeat (simpl; red; mred). }
+            { mred; apply H7; auto. }
+        + red in H6; red; simpl in *; mred; simpl.
+          destruct (oss@[child1Idx]) as [cost1|] eqn:Hcost1; simpl in *; [|auto].
+          destruct (oss@[child2Idx]) as [cost2|] eqn:Hcost2; simpl in *; [|auto].
+          destruct (orqs@[child1Idx]) as [corq1|] eqn:Hcorq1; simpl in *; [|auto].
+          destruct (orqs@[child2Idx]) as [corq2|] eqn:Hcorq2; simpl in *; [|auto].
+          destruct H6 as [[cv ?] ?].
+          red in H6; dest.
+          unfold getDir in *; simpl in *.
+          disc_rule_conds_ex.
+          destruct H6 as [|[|]];
+            [exfalso; solve_rule_conds_ex
+            | |exfalso; destruct H6 as [? [|]]; solve_rule_conds_ex].
+          
+          split.
+          * exists cv.
+            repeat ssplit.
+            { solve_rule_conds_ex.
+              right; left.
+              unfold msiM, msiS, msiI in *; lia.
+            }
+            { solve_rule_conds_ex. }
+            { solve_rule_conds_ex. }
+            { solve_rule_conds_ex. }
+          * disc_rule_conds_ex.
+            assert (In (child child1Idx ec1 ce1 c1pRq c1pRs pc1) (sys_objs impl))
+              by (simpl; tauto).
+            good_locking_get (child child1Idx ec1 ce1 c1pRq c1pRs pc1).
+            clear H6.
+            eapply upLockInvORq_rqUp_length_one_locked in H28; try reflexivity;
+              [|eapply findQ_length_ge_one; apply FirstMP_InMP; eassumption].
+            solve_rule_conds_ex.
+
+      - (** [parentEvictRqImmLastS] *)
+        disc_rule_conds_ex.
+
+        split.
+        + split.
+          * apply Forall_app.
+            { apply forall_removeOnce.
+              eapply atomic_rqUp_preserves_msg_out_preds with (oidx:= child1Idx);
+                [exact msiSv_impl_ORqsInit
+                |exact msiSv_impl_RqRsSys|..]; eauto.
+              { intro; dest_in; discriminate. }
+              { red; auto. }
+              { exact msiSvMsgOutPred_good. }
+            }
+            { repeat (constructor; simpl).
+              red; repeat (simpl; mred).
+              lia.
+            }
+          * red; simpl; intros.
+            icase oidx.
+            { repeat (simpl; red; mred). }
+            { mred; apply H7; auto. }
+        + red in H6; red; simpl in *; mred; simpl.
+          destruct (oss@[child1Idx]) as [cost1|] eqn:Hcost1; simpl in *; [|auto].
+          destruct (oss@[child2Idx]) as [cost2|] eqn:Hcost2; simpl in *; [|auto].
+          destruct (orqs@[child1Idx]) as [corq1|] eqn:Hcorq1; simpl in *; [|auto].
+          destruct (orqs@[child2Idx]) as [corq2|] eqn:Hcorq2; simpl in *; [|auto].
+          destruct H6 as [[cv ?] ?].
+          red in H6; dest.
+          unfold getDir in *; simpl in *.
+          disc_rule_conds_ex.
+          destruct H6 as [|[|]];
+            [exfalso; solve_rule_conds_ex
+            | |exfalso; destruct H6 as [? [|]]; solve_rule_conds_ex].
+          
+          split.
+          * exists cv.
+            repeat ssplit.
+            { solve_rule_conds_ex. }
+            { solve_rule_conds_ex. }
+            { solve_rule_conds_ex. }
+            { solve_rule_conds_ex. }
+          * disc_rule_conds_ex.
+            assert (In (child child1Idx ec1 ce1 c1pRq c1pRs pc1) (sys_objs impl))
+              by (simpl; tauto).
+            good_locking_get (child child1Idx ec1 ce1 c1pRq c1pRs pc1).
+            clear H6.
+            eapply upLockInvORq_rqUp_length_one_locked in H28; try reflexivity;
+              [|eapply findQ_length_ge_one; apply FirstMP_InMP; eassumption].
+            solve_rule_conds_ex.
+
+      - (** [parentEvictRqImmM] *)
+        disc_rule_conds_ex.
+
+        split.
+        + split.
+          * apply Forall_app.
+            { apply forall_removeOnce.
+              eapply atomic_rqUp_preserves_msg_out_preds with (oidx:= child1Idx);
+                [exact msiSv_impl_ORqsInit
+                |exact msiSv_impl_RqRsSys|..]; eauto.
+              { intro; dest_in; discriminate. }
+              { red; auto. }
+              { exact msiSvMsgOutPred_good. }
+            }
+            { repeat (constructor; simpl).
+              red; repeat (simpl; mred).
+              lia.
+            }
+          * red; simpl; intros.
+            icase oidx.
+            { repeat (simpl; red; mred). }
+            { mred; apply H7; auto. }
+        + red in H6; red; simpl in *; mred; simpl.
+          destruct (oss@[child1Idx]) as [cost1|] eqn:Hcost1; simpl in *; [|auto].
+          destruct (oss@[child2Idx]) as [cost2|] eqn:Hcost2; simpl in *; [|auto].
+          destruct (orqs@[child1Idx]) as [corq1|] eqn:Hcorq1; simpl in *; [|auto].
+          destruct (orqs@[child2Idx]) as [corq2|] eqn:Hcorq2; simpl in *; [|auto].
+          destruct H6 as [[cv ?] ?].
+          red in H6; dest.
+          unfold getDir in *; simpl in *.
+          disc_rule_conds_ex.
+          destruct H6 as [|[|]]; try (exfalso; solve_rule_conds_ex; fail).
+
+          assert (In (child child1Idx ec1 ce1 c1pRq c1pRs pc1) (sys_objs impl))
+            by (simpl; tauto).
+          good_locking_get (child child1Idx ec1 ce1 c1pRq c1pRs pc1).
+          clear H26.
+          eapply upLockInvORq_rqUp_length_one_locked in H27; try reflexivity;
+            [|eapply findQ_length_ge_one; apply FirstMP_InMP; eassumption].
+          disc_rule_conds_ex.
+          
+          split.
+          * exists n.
+            repeat ssplit.
+            { solve_rule_conds_ex.
+              left.
+              unfold msiM, msiS, msiI in *; lia.
+            }
+            { solve_rule_conds_ex. }
+            { solve_rule_conds_ex.
+              unfold msiM, msiS, msiI in *; lia.
+            }
+            { solve_rule_conds_ex. }
+          * solve_rule_conds_ex.
+
+      (** parent(child2) *)
+
+      - (** [parentGetRqImm] *)
+        disc_rule_conds_ex.
+
+        split.
+        + split.
+          * apply Forall_app.
+            { apply forall_removeOnce.
+              eapply atomic_rqUp_preserves_msg_out_preds with (oidx:= child2Idx);
+                [exact msiSv_impl_ORqsInit
+                |exact msiSv_impl_RqRsSys|..]; eauto.
+              { intro; dest_in; discriminate. }
+              { red; auto. }
+              { exact msiSvMsgOutPred_good. }
+            }
+            { repeat (constructor; simpl).
+              red; repeat (simpl; mred).
+            }
+          * red; simpl; intros.
+            icase oidx.
+            { repeat (simpl; red; mred). }
+            { mred; apply H7; auto. }
+        + red in H6; red; simpl in *; mred; simpl.
+          destruct (oss@[child1Idx]) as [cost1|] eqn:Hcost1; simpl in *; [|auto].
+          destruct (oss@[child2Idx]) as [cost2|] eqn:Hcost2; simpl in *; [|auto].
+          destruct (orqs@[child1Idx]) as [corq1|] eqn:Hcorq1; simpl in *; [|auto].
+          destruct (orqs@[child2Idx]) as [corq2|] eqn:Hcorq2; simpl in *; [|auto].
+          destruct H6 as [[cv ?] ?].
+          red in H6; dest.
+          split.
+          * exists cv.
+            clear H8.
+            red; repeat ssplit.
+            { solve_rule_conds_ex.
+              right; left.
+              destruct H6 as [|[|]].
+              { solve_rule_conds_ex.
+                unfold msiM, msiS, msiI in *; lia.
+              }
+              { solve_rule_conds_ex. }
+              { unfold msiM, msiS, msiI in *; lia. }
+            }
+            { solve_rule_conds_ex. }
+            { solve_rule_conds_ex. }
+            { solve_rule_conds_ex. }
+          * disc_rule_conds_ex.
+            assert (In (child child2Idx ec2 ce2 c2pRq c2pRs pc2) (sys_objs impl))
+              by (simpl; tauto).
+            good_locking_get (child child2Idx ec2 ce2 c2pRq c2pRs pc2).
+            clear H24.
+            eapply upLockInvORq_rqUp_length_one_locked in H26; try reflexivity;
+              [|eapply findQ_length_ge_one; apply FirstMP_InMP; eassumption].
+            solve_rule_conds_ex.
+
+      - (** [parentGetDownRqS] *)
+        disc_rule_conds_ex.
+
+        split.
+        + split.
+          * apply Forall_app.
+            { apply forall_removeOnce.
+              eapply atomic_rqUp_preserves_msg_out_preds with (oidx:= child2Idx);
+                [exact msiSv_impl_ORqsInit
+                |exact msiSv_impl_RqRsSys|..]; eauto.
+              { intro; dest_in; discriminate. }
+              { red; auto. }
+              { exact msiSvMsgOutPred_good. }
+            }
+            { repeat (constructor; simpl). }
+          * red; simpl; intros.
+            icase oidx.
+            { repeat (simpl; red; mred).
+              simpl; right; auto.
+            }
+            { mred; apply H7; auto. }
+        + red in H6; red; simpl in *; mred; simpl.
+          destruct (oss@[child1Idx]) as [cost1|]; simpl in *; [|auto].
+          destruct (oss@[child2Idx]) as [cost2|]; simpl in *; [|auto].
+          destruct (orqs@[child1Idx]) as [corq1|]; simpl in *; [|auto].
+          destruct (orqs@[child2Idx]) as [corq2|]; simpl in *; [|auto].
+          destruct H6 as [[cv ?] ?].
+          red in H6; dest.
+          split.
+          * exists cv.
+            clear H8.
+            red; repeat ssplit.
+            { solve_rule_conds_ex. }
+            { solve_rule_conds_ex. }
+            { solve_rule_conds_ex. }
+            { solve_rule_conds_ex. }
+          * solve_rule_conds_ex.
+
+      - (** [parentSetRqImm] *)
+        disc_rule_conds_ex.
+
+        split.
+        + split.
+          * apply Forall_app.
+            { apply forall_removeOnce.
+              eapply atomic_rqUp_preserves_msg_out_preds with (oidx:= child2Idx);
+                [exact msiSv_impl_ORqsInit
+                |exact msiSv_impl_RqRsSys|..]; eauto.
+              { intro; dest_in; discriminate. }
+              { red; auto. }
+              { exact msiSvMsgOutPred_good. }
+            }
+            { repeat (constructor; simpl).
+              red; repeat (simpl; mred).
+            }
+          * red; simpl; intros.
+            icase oidx.
+            { repeat (simpl; red; mred). }
+            { mred; apply H7; auto. }
+        + red in H6; red; simpl in *; mred; simpl.
+          destruct (oss@[child1Idx]) as [cost1|] eqn:Hcost1; simpl in *; [|auto].
+          destruct (oss@[child2Idx]) as [cost2|] eqn:Hcost2; simpl in *; [|auto].
+          destruct (orqs@[child1Idx]) as [corq1|] eqn:Hcorq1; simpl in *; [|auto].
+          destruct (orqs@[child2Idx]) as [corq2|] eqn:Hcorq2; simpl in *; [|auto].
+          destruct H6 as [[cv ?] ?].
+          red in H6; dest.
+          unfold getDir in H14; simpl in H14.
+          split.
+          * exists cv.
+            red; repeat ssplit.
+            { solve_rule_conds_ex. }
+            { solve_rule_conds_ex. }
+            { solve_rule_conds_ex. }
+            { solve_rule_conds_ex. }
+          * disc_rule_conds_ex.
+            assert (In (child child2Idx ec2 ce2 c2pRq c2pRs pc2) (sys_objs impl))
+              by (simpl; tauto).
+            good_locking_get (child child2Idx ec2 ce2 c2pRq c2pRs pc2).
+            clear H24.
+            eapply upLockInvORq_rqUp_length_one_locked in H26; try reflexivity;
+              [|eapply findQ_length_ge_one; apply FirstMP_InMP; eassumption].
+            solve_rule_conds_ex.
+
+      - (** [parentSetDownRqM] *)
+        disc_rule_conds_ex.
+
+        split.
+        + split.
+          * apply Forall_app.
+            { apply forall_removeOnce.
+              eapply atomic_rqUp_preserves_msg_out_preds with (oidx:= child2Idx);
+                [exact msiSv_impl_ORqsInit
+                |exact msiSv_impl_RqRsSys|..]; eauto.
+              { intro; dest_in; discriminate. }
+              { red; auto. }
+              { exact msiSvMsgOutPred_good. }
+            }
+            { repeat (constructor; simpl). }
+          * red; simpl; intros.
+            icase oidx.
+            { repeat (simpl; red; mred).
+              simpl; right; auto.
+            }
+            { mred; apply H7; auto. }
+        + red in H6; red; simpl in *; mred; simpl.
+          destruct (oss@[child1Idx]) as [cost1|]; simpl in *; [|auto].
+          destruct (oss@[child2Idx]) as [cost2|]; simpl in *; [|auto].
+          destruct (orqs@[child1Idx]) as [corq1|]; simpl in *; [|auto].
+          destruct (orqs@[child2Idx]) as [corq2|]; simpl in *; [|auto].
+          destruct H6 as [[cv ?] ?].
+          red in H6; dest.
+          split.
+          * exists cv.
+            clear H8.
+            red; repeat ssplit.
+            { solve_rule_conds_ex. }
+            { solve_rule_conds_ex. }
+            { solve_rule_conds_ex. }
+            { solve_rule_conds_ex. }
+          * solve_rule_conds_ex.
+
+      - (** [parentGetDownRsS] *)
+        disc_rule_conds_ex.
+
+        obj_visited_rsUp parentIdx child1Idx.
+        disc_lock_preds parentIdx.
+        disc_rule_conds_ex.
+        destruct H11; dest; [discriminate|].
+        clear H11.
+        disc_rule_conds_ex.
+
+        (* discharge message predicates *)
+        disc_msg_preds H4.
+        disc_rule_conds_ex.
+        
+        split.
+        + split.
+          * apply Forall_app.
+            { apply forall_removeOnce.
+              eapply atomic_rsUps_preserves_msg_out_preds
+                with (rsUps:= [(c1pRs, rmsg)]); eauto.
+              { exact msiSv_impl_ORqsInit. }
+              { exact msiSv_impl_RqRsSys. }
+              { repeat constructor; intro; dest_in. }
+              { apply SubList_cons; [|apply SubList_nil].
+                assumption.
+              }
+              { instantiate (1:= fun _ => True).
+                instantiate (1:= [pc1]).
+                repeat split.
+                { discriminate. }
+                { repeat constructor.
+                  simpl; exists child1Idx.
+                  repeat split.
+                }
+              }
+              { exact msiSvMsgOutPred_good. }
+            }
+            { repeat (constructor; simpl).
+              red; simpl.
+              solve_rule_conds_ex.
+            }
+          * red; simpl; intros.
+            icase oidx.
+            { repeat (simpl; red; mred). }
+            { mred; apply H7; auto. }
+        + red in H6; red; simpl in *; mred; simpl.
+          destruct (oss@[child2Idx]) as [cost2|] eqn:Hcost2; simpl in *; [|auto].
+          destruct (orqs@[child1Idx]) as [corq1|] eqn:Hcorq1; simpl in *; [|auto].
+          destruct (orqs@[child2Idx]) as [corq2|] eqn:Hcorq2; simpl in *; [|auto].
+          destruct H6 as [[cv ?] ?].
+          red in H6; dest.
+
+          assert (In (child child2Idx ec2 ce2 c2pRq c2pRs pc2) (sys_objs impl))
+            by (simpl; tauto).
+          good_locking_get (child child2Idx ec2 ce2 c2pRq c2pRs pc2).
+          clear H24.
+          eapply upLockInvORq_parent_locked_locked in H26; try reflexivity;
+            [|red; repeat (simpl; mred); eauto]; dest.
+          
+          split.
+          * exists val0.
+            clear H11.
+            red; repeat ssplit.
+            { solve_rule_conds_ex.
+              right; left; auto.
+            }
+            { solve_rule_conds_ex. }
+            { solve_rule_conds_ex. }
+            { solve_rule_conds_ex. }
+          * solve_rule_conds_ex.
+
+      - (** [parentSetDownRsM] *)
+        disc_rule_conds_ex.
+
+        obj_visited_rsUp parentIdx child1Idx.
+        disc_lock_preds parentIdx.
+        disc_rule_conds_ex.
+        destruct H11; dest; [discriminate|].
+        clear H11.
+        disc_rule_conds_ex.
+
+        (* discharge message predicates *)
+        disc_msg_preds H4.
+        disc_rule_conds_ex.
+        
+        split.
+        + split.
+          * apply Forall_app.
+            { apply forall_removeOnce.
+              eapply atomic_rsUps_preserves_msg_out_preds
+                with (rsUps:= [(c1pRs, rmsg)]); eauto.
+              { exact msiSv_impl_ORqsInit. }
+              { exact msiSv_impl_RqRsSys. }
+              { repeat constructor; intro; dest_in. }
+              { apply SubList_cons; [|apply SubList_nil].
+                assumption.
+              }
+              { instantiate (1:= fun _ => True).
+                instantiate (1:= [pc1]).
+                repeat split.
+                { discriminate. }
+                { repeat constructor.
+                  simpl; exists child1Idx.
+                  repeat split.
+                }
+              }
+              { exact msiSvMsgOutPred_good. }
+            }
+            { repeat (constructor; simpl).
+              red; simpl.
+              solve_rule_conds_ex.
+            }
+          * red; simpl; intros.
+            icase oidx.
+            { repeat (simpl; red; mred). }
+            { mred; apply H7; auto. }
+        + red in H6; red; simpl in *; mred; simpl.
+          destruct (oss@[child2Idx]) as [cost2|] eqn:Hcost1; simpl in *; [|auto].
+          destruct (orqs@[child1Idx]) as [corq1|] eqn:Hcorq1; simpl in *; [|auto].
+          destruct (orqs@[child2Idx]) as [corq2|] eqn:Hcorq2; simpl in *; [|auto].
+          destruct H6 as [[cv ?] ?].
+          red in H6; dest.
+
+          assert (In (child child2Idx ec2 ce2 c2pRq c2pRs pc2) (sys_objs impl))
+            by (simpl; tauto).
+          good_locking_get (child child2Idx ec2 ce2 c2pRq c2pRs pc2).
+          clear H24.
+          eapply upLockInvORq_parent_locked_locked in H26; try reflexivity;
+            [|red; repeat (simpl; mred); eauto]; dest.
+
+          split.
+          * exists val0.
+            clear H11.
+            red; repeat ssplit.
+            { solve_rule_conds_ex. }
+            { solve_rule_conds_ex. }
+            { solve_rule_conds_ex. }
+            { solve_rule_conds_ex. }
+          * solve_rule_conds_ex.
+
+      - (** [parentEvictRqImmS] *)
+        disc_rule_conds_ex.
+
+        split.
+        + split.
+          * apply Forall_app.
+            { apply forall_removeOnce.
+              eapply atomic_rqUp_preserves_msg_out_preds with (oidx:= child2Idx);
+                [exact msiSv_impl_ORqsInit
+                |exact msiSv_impl_RqRsSys|..]; eauto.
+              { intro; dest_in; discriminate. }
+              { red; auto. }
+              { exact msiSvMsgOutPred_good. }
+            }
+            { repeat (constructor; simpl).
+              red; repeat (simpl; mred).
+              red in H6; simpl in H6.
+              unfold getDir in *; simpl in *.
+              disc_rule_conds_ex.
+              destruct H6 as [|[|]]; dest.
+              { exfalso; solve_rule_conds_ex. }
+              { subst; auto. }
+              { exfalso; destruct H26; solve_rule_conds_ex. }
+            }
+          * red; simpl; intros.
+            icase oidx.
+            { repeat (simpl; red; mred). }
+            { mred; apply H7; auto. }
+        + red in H6; red; simpl in *; mred; simpl.
+          destruct (oss@[child1Idx]) as [cost1|] eqn:Hcost1; simpl in *; [|auto].
+          destruct (oss@[child2Idx]) as [cost2|] eqn:Hcost2; simpl in *; [|auto].
+          destruct (orqs@[child1Idx]) as [corq1|] eqn:Hcorq1; simpl in *; [|auto].
+          destruct (orqs@[child2Idx]) as [corq2|] eqn:Hcorq2; simpl in *; [|auto].
+          destruct H6 as [[cv ?] ?].
+          red in H6; dest.
+          unfold getDir in *; simpl in *.
+          disc_rule_conds_ex.
+          destruct H6 as [|[|]];
+            [exfalso; solve_rule_conds_ex
+            | |exfalso; destruct H6 as [? [|]]; solve_rule_conds_ex].
+          
+          split.
+          * exists cv.
+            repeat ssplit.
+            { solve_rule_conds_ex.
+              right; left.
+              unfold msiM, msiS, msiI in *; lia.
+            }
+            { solve_rule_conds_ex. }
+            { solve_rule_conds_ex. }
+            { solve_rule_conds_ex. }
+          * disc_rule_conds_ex.
+            assert (In (child child2Idx ec2 ce2 c2pRq c2pRs pc2) (sys_objs impl))
+              by (simpl; tauto).
+            good_locking_get (child child2Idx ec2 ce2 c2pRq c2pRs pc2).
+            clear H6.
+            eapply upLockInvORq_rqUp_length_one_locked in H28; try reflexivity;
+              [|eapply findQ_length_ge_one; apply FirstMP_InMP; eassumption].
+            solve_rule_conds_ex.
+
+      - (** [parentEvictRqImmLastS] *)
+        disc_rule_conds_ex.
+
+        split.
+        + split.
+          * apply Forall_app.
+            { apply forall_removeOnce.
+              eapply atomic_rqUp_preserves_msg_out_preds with (oidx:= child2Idx);
+                [exact msiSv_impl_ORqsInit
+                |exact msiSv_impl_RqRsSys|..]; eauto.
+              { intro; dest_in; discriminate. }
+              { red; auto. }
+              { exact msiSvMsgOutPred_good. }
+            }
+            { repeat (constructor; simpl).
+              red; repeat (simpl; mred).
+              lia.
+            }
+          * red; simpl; intros.
+            icase oidx.
+            { repeat (simpl; red; mred). }
+            { mred; apply H7; auto. }
+        + red in H6; red; simpl in *; mred; simpl.
+          destruct (oss@[child1Idx]) as [cost1|] eqn:Hcost1; simpl in *; [|auto].
+          destruct (oss@[child2Idx]) as [cost2|] eqn:Hcost2; simpl in *; [|auto].
+          destruct (orqs@[child1Idx]) as [corq1|] eqn:Hcorq1; simpl in *; [|auto].
+          destruct (orqs@[child2Idx]) as [corq2|] eqn:Hcorq2; simpl in *; [|auto].
+          destruct H6 as [[cv ?] ?].
+          red in H6; dest.
+          unfold getDir in *; simpl in *.
+          disc_rule_conds_ex.
+          destruct H6 as [|[|]];
+            [exfalso; solve_rule_conds_ex
+            | |exfalso; destruct H6 as [? [|]]; solve_rule_conds_ex].
+          
+          split.
+          * exists cv.
+            repeat ssplit.
+            { solve_rule_conds_ex. }
+            { solve_rule_conds_ex. }
+            { solve_rule_conds_ex. }
+            { solve_rule_conds_ex. }
+          * disc_rule_conds_ex.
+            assert (In (child child2Idx ec2 ce2 c2pRq c2pRs pc2) (sys_objs impl))
+              by (simpl; tauto).
+            good_locking_get (child child2Idx ec2 ce2 c2pRq c2pRs pc2).
+            clear H6.
+            eapply upLockInvORq_rqUp_length_one_locked in H28; try reflexivity;
+              [|eapply findQ_length_ge_one; apply FirstMP_InMP; eassumption].
+            solve_rule_conds_ex.
+
+      - (** [parentEvictRqImmM] *)
+        disc_rule_conds_ex.
+
+        split.
+        + split.
+          * apply Forall_app.
+            { apply forall_removeOnce.
+              eapply atomic_rqUp_preserves_msg_out_preds with (oidx:= child2Idx);
+                [exact msiSv_impl_ORqsInit
+                |exact msiSv_impl_RqRsSys|..]; eauto.
+              { intro; dest_in; discriminate. }
+              { red; auto. }
+              { exact msiSvMsgOutPred_good. }
+            }
+            { repeat (constructor; simpl).
+              red; repeat (simpl; mred).
+              lia.
+            }
+          * red; simpl; intros.
+            icase oidx.
+            { repeat (simpl; red; mred). }
+            { mred; apply H7; auto. }
+        + red in H6; red; simpl in *; mred; simpl.
+          destruct (oss@[child1Idx]) as [cost1|] eqn:Hcost1; simpl in *; [|auto].
+          destruct (oss@[child2Idx]) as [cost2|] eqn:Hcost2; simpl in *; [|auto].
+          destruct (orqs@[child1Idx]) as [corq1|] eqn:Hcorq1; simpl in *; [|auto].
+          destruct (orqs@[child2Idx]) as [corq2|] eqn:Hcorq2; simpl in *; [|auto].
+          destruct H6 as [[cv ?] ?].
+          red in H6; dest.
+          unfold getDir in *; simpl in *.
+          disc_rule_conds_ex.
+          destruct H6 as [|[|]]; try (exfalso; solve_rule_conds_ex; fail).
+
+          assert (In (child child2Idx ec2 ce2 c2pRq c2pRs pc2) (sys_objs impl))
+            by (simpl; tauto).
+          good_locking_get (child child2Idx ec2 ce2 c2pRq c2pRs pc2).
+          clear H26.
+          eapply upLockInvORq_rqUp_length_one_locked in H27; try reflexivity;
+            [|eapply findQ_length_ge_one; apply FirstMP_InMP; eassumption].
+          disc_rule_conds_ex.
+          
+          split.
+          * exists n.
+            repeat ssplit.
+            { solve_rule_conds_ex.
+              left.
+              unfold msiM, msiS, msiI in *; lia.
+            }
+            { solve_rule_conds_ex.
+              unfold msiM, msiS, msiI in *; lia.
+            }
+            { solve_rule_conds_ex. }
+            { solve_rule_conds_ex. }
+          * solve_rule_conds_ex.
+
+    Qed.
+
+    Lemma ImplStateInv_init:
+      ImplStateInv (initsOf impl).
+    Proof.
+      red; simpl.
+      unfold implOStatesInit, implORqsInit; mred.
+      simpl.
+      repeat split.
+      exists 0.
+      repeat split; intros.
+      - vm_compute; intros.
+        right; left; auto.
+      - discriminate.
+      - discriminate.
+    Qed.
+
+    Lemma ImplStateInv_invStep:
+      InvStep impl step_m ImplStateInv.
+    Proof.
+      apply invSeq_serializable_invStep.
+      - apply ImplStateInv_init.
+      - apply inv_trs_seqSteps.
+        apply msiSv_impl_InvTrs.
+      - eapply rqrs_Serializable.
+        + apply msiSv_impl_ORqsInit.
+        + apply msiSv_impl_RqRsSys.
+    Qed.
+
+  End Facts.
+  
+End Inv.
+
